improvements

MergeSort.fst
@@ -1,118 +1,46 @@
+(**This module implements a generic merge sort and proves it's stability.**)
 module MergeSort
+(**@author A Manning**)
+
 open FStar.List.Tot
 open GenericSort
 open GenericStability
 
-val merge: #a:eqtype
-  -> l_0:list a{is_Cons l_0}
-  -> l_1:list a{is_Cons l_1}
-  -> key:(a -> Tot int){sorted l_0 key /\ sorted l_1 key}
-  -> l':list a{sorted l' key /\ permutation_2 l' l_0 l_1}
+(** The key function k will appear frequently here.**)
 
-let rec merge #a l_0 l_1 key =
-  let h_0 = hd l_0 in
-  let h_1 = hd l_1 in
-  if ((key h_0) <= (key h_1)) then
-    if tl l_0 = [] then (h_0::l_1)
-    else
-    (cons_sorted h_0 (merge (tl l_0) l_1 key) key;
-    h_0::(merge (tl l_0) l_1 key))
-  else if tl l_1 = [] then (h_1::l_0)
-    else
-    cons_sorted h_1 (merge l_0 (tl l_1) key) key;
-    h_1::(merge l_0 (tl l_1) key)
-(*)
-  match ((key h_0) <= (key h_1)) with
-  | true ->
-    cons_sorted h_0 (merge (tl l_0) l_1 key) key;
-    h_0::(merge (tl l_0) l_1 key)
-  | false ->
-      cons_sorted h_1 (merge l_0 (tl l_1) key) key;
-      h_1::(merge l_0 (tl l_1) key)
-
-(*)
-val ms: #a:eqtype -> l_0:list a -> key:(a -> Tot int) -> l':list a
-let ms #a l_0 key =
-  match l_0 with
-  | [] | [_] -> l_0
-  | [a_0;a_1] -> (if key a_0 <= key a_1 then [a_0;a_1] else [a_1;a_0])
-  | [a_0;a_1;a_2] -> []
-
-
-
-
-
-
-
-
-
-
-
-
-
-
-
-
-
-
-
-
-
-
-
-
-
-(*)
-type split_inv (#a:eqtype) (l:list a) (l1:list a) (l2:list a) (key:(a -> Tot int)) =
-    permutation_2 l l1 l2 /\
-    (* needed for decreases clause in mergesort function *)
-    length l > length l1 /\ length l > length l2
-    /\ (forall x y.
-    (appears_before x y l ==>
-    appears_before x y l1
-    \/ appears_before x y l2
-    \/ ~(mem x l1 /\ mem y l1 )))
-
-
-val split: (#a:eqtype) -> l:list a -> Tot r:(list a * list a)
-  (requires (is_Cons l /\ is_Cons (Cons.tl l)))
-	(ensures (split_inv l (fst r) (snd r)))
-let rec split (x::y::l) =
-  match l with
-    | [] -> [x], [y]
-    | [x'] -> x::y, [x']
-    | _ -> let l1, l2 = split l in
-           x::l1, y::l2
-(*)
-(* Verification succeeds even without this invariant;
-   it just takes a lot longer (22s vs 7s) *)
-type merge_inv (l1:list int) (l2:list int) (l:list int) =
-    (is_Cons l1 /\ is_Cons l /\ Cons.hd l1 = Cons.hd l) \/
-    (is_Cons l2 /\ is_Cons l /\ Cons.hd l2 = Cons.hd l) \/
-    (is_Nil l1 /\ is_Nil l2 /\ is_Nil l)
-
-val merge: l1:list int -> l2:list int -> Pure (list int)
-             (requires (sorted l1 /\ sorted l2))
-             (ensures (fun l -> sorted l /\ permutation_2 l l1 l2
-                                         /\ merge_inv l1 l2 l
-                                         /\ (forall x y. ((appears_before x y l1 ==>
-                                          appears_before x y l)
-                                          /\(appears_before x y l2 ==>
-                                          appears_before x y l)))))
-let rec merge l1 l2 = match (l1, l2) with
+(**First define the merge function without any properties.**)
+val merge': #a:eqtype -> (l1:list a) -> (l2:list a) -> k:(a -> Tot int) -> Tot (list a)
+let rec merge' #a l1 l2 k = match (l1, l2) with
   | [], _ -> l2
   | _, [] -> l1
-  | h1::tl1, h2::tl2 -> if h1 <= h2
-                        then h1::(merge tl1 l2)
-                        else h2::(merge l1 tl2)
-(*)
-val mergesort: l:list int -> Pure (list int) (requires True)
-      (ensures (fun r -> sorted r /\ permutation l r)) (decreases (length l))
-let rec mergesort l = match l with
-  | [] -> []
-  | [x] -> [x]
-  | _ ->
-    let (l1, l2) = split l in
-    let sl1 = mergesort l1 in
-    let sl2 = mergesort l2 in
-    merge sl1 sl2
+  | h1::tl1, h2::tl2 -> if k h1 <= k h2
+                        then h1::(merge' tl1 l2 k)
+                        else h2::(merge' l1 tl2 k)
+
+
+val merge'_permutation: #a:eqtype ->
+  (l1:list a) ->
+  (l2:list a) ->
+  k:(a -> Tot int) ->
+  Lemma(ensures permutation_2 (merge' l1 l2 k) l1 l2)
+
+let rec merge'_permutation #a l1 l2 k = match (l1, l2) with
+  | [], _ -> ()
+  | _, [] -> ()
+  | h1::tl1, h2::tl2 -> if k h1 <= k h2
+                          then (merge'_permutation tl1 l2 k)
+                        else (merge'_permutation l1 tl2 k)
+
+val merge'_sorted: #a:eqtype ->
+  (l1:list a) ->
+  (l2:list a) ->
+  k:(a -> Tot int) ->
+  Lemma(requires (sorted l1 k /\ sorted l2 k))
+    (ensures sorted (merge' l1 l2 k) k)
+let rec merge'_sorted #a l1 l2 k = merge'_permutation l1 l2 k;
+match (l1, l2) with
+  | [], _ -> ()
+  | _, [] -> ()
+  | h1::tl1, h2::tl2 -> if k h1 <= k h2
+                          then (merge'_sorted tl1 l2 k)
+                        else (merge'_sorted l1 tl2 k)
